src/program_proof/fencing/config_proof.v
@@ -1,0 +1,36 @@
+From Perennial.program_proof Require Import grove_prelude.
+From Goose.github_com.mit_pdos.gokv.fencing Require Import frontend.
+From Perennial.program_proof Require Import grove_prelude.
+From Perennial.program_proof.memkv Require Export urpc_lib urpc_proof urpc_spec.
+From Perennial.program_proof.fencing Require Export ctr_proof.
+From iris.base_logic Require Import mono_nat.
+
+Section config_proof.
+Context `{!heapGS Σ}.
+
+Record config_names :=
+  {
+
+  }.
+
+Implicit Type γ:config_names.
+
+Definition is_config_host γ (host:u64) : iProp Σ.
+Admitted.
+
+Definition own_ConfigClerk γ (ck:loc) : iProp Σ.
+Admitted.
+
+Lemma wp_MakeClerk γ host :
+  is_config_host γ host -∗
+  {{{
+        True
+  }}}
+    config.MakeClerk #host
+  {{{
+        (ck:loc), RET #ck; own_ConfigClerk γ ck
+  }}}.
+Proof.
+Admitted.
+
+End config_proof.
